feat: verify rho

lean/Shars/Verification/Rho.lean
@@ -12,6 +12,7 @@ import Shars.Verification.Auxiliary
 
 set_option maxHeartbeats 1000000
 attribute [-simp] List.getElem!_eq_getElem?_getD
+attribute [ext (iff := false)] List.ext_getElem!
 attribute [simp] Aeneas.Std.Slice.set
 
 open Aeneas hiding Std.Array
@@ -21,16 +22,15 @@ def Spec.Keccak.ρ.sequence_point(n: Nat): Fin 5 × Fin 5 := n.repeat (fun (x,y)
 
 def Spec.Keccak.ρ.sequence := Vector.range 24 |>.map sequence_point
 
-
 @[progress]
-theorem algos.rho_offset.spec (t : Std.Usize)
+theorem algos.rho.offset.spec (t : Std.U32)
 : t.val < 24
 → ∃ output,
-  rho_offset t = .ok output ∧
+  offset t = .ok output ∧
   output.val = (@Spec.Keccak.ρ.offset 6 t.val).val
 := by
   intro bounded
-  unfold rho_offset Spec.Keccak.ρ.offset
+  unfold rho.offset Spec.Keccak.ρ.offset
   progress* by scalar_tac
   · calc i.val * i1.val
     _ ≤ 24 * i1.val := by
@@ -39,8 +39,8 @@ theorem algos.rho_offset.spec (t : Std.Usize)
     _ ≤ 24 * 25 := by
       apply Nat.mul_le_mul_left
       scalar_tac
-    _ ≤ Std.Usize.max := by scalar_tac
-  simp [*]
+    _ ≤ _ := by scalar_tac
+  simp [*, Spec.w]
 
 def Spec.Keccak.ρ.inner_loop(input res: Spec.Keccak.StateArray 6)(t: Fin 24)(x y: Fin 5)(z: Nat) := Id.run do
   let mut res' := res
@@ -48,92 +48,421 @@ def Spec.Keccak.ρ.inner_loop(input res: Spec.Keccak.StateArray 6)(t: Fin 24)(x 
     res' := res'.set x y z.val <| input.get x y (z - Spec.Keccak.ρ.offset t)
   return res'
 
-def Spec.Keccak.ρ.loop(input res: Spec.Keccak.StateArray 6)(t : Nat)(x y: Fin 5) := Id.run do
-  let mut (x',y') := (x,y)
-  let mut res' := res
-  for t in List.finRange 24 |>.drop t do
-    res' := ρ.inner_loop input res' t x' y' 0
-    (x',y') := (y', 2*x' + 3*y')
-  return res'
+def IR.rho.bitmangling(state res: List Bool)(x y offset: Nat)(z_start: Nat := 0): List Bool := Id.run do
+  let mut res := res
+  for z in [z_start:Spec.w 6] do
+    res := res.set (IR.encodeIndex x y z) <| state[IR.encodeIndex x y ((z + Spec.w 6 - offset % Spec.w 6) % Spec.w 6)]!
+  return res
 
-theorem Spec.Keccak.ρ.loop.spec(input: Spec.Keccak.StateArray 6)
-: ρ.loop input input 0 1 0 = ρ input
-:= by simp [ρ,ρ.loop, ρ.inner_loop]
-
--- example(x: Nat)(x_lt: x < n)(eq: n = m): Fin.cast eq ⟨x, x_lt⟩ = ⟨x, eq ▸ x_lt⟩ := by
---   rfl
-
-@[progress]
-theorem algos.rho.inner_loop.spec(input res : StateArray) (t x y z : Std.Usize)
-: t.val < 24
-→ x.val < 5
-→ y.val < 5
-→ z.val ≤ Spec.w 6
-→ ∃ output,
-  rho.inner_loop res input t x y z = .ok output ∧
-  output.toSpec = Spec.Keccak.ρ.inner_loop input.toSpec res.toSpec t.val.cast x.val.cast y.val.cast z.val.cast
+theorem IR.rho.length_bitmangling(state res: List Bool)(x y offset: Nat)
+: (bitmangling state res x y offset).length = res.length
 := by
-  intro t_lt x_lt y_lt z_lt
-  rw [rho.inner_loop, Spec.Keccak.ρ.inner_loop]
-  split
-  . let* ⟨ i, i_post ⟩ ← rho_offset.spec
-    let* ⟨ i1, i1_post ⟩ ← Std.Usize.sub_spec'
-    let* ⟨ i2, i2_post ⟩ ← Std.Usize.add_spec
-    let* ⟨ z2, z2_post ⟩ ← Std.Usize.rem_spec
-    let* ⟨ b, b_post ⟩ ← StateArray.index.spec
-    let* ⟨ x_1, x_2, x_post_1, x_post_2 ⟩ ← StateArray.index_mut.spec
-    let* ⟨ z1, z1_post ⟩ ← Std.Usize.add_spec
-    let* ⟨ res, res_post ⟩ ← spec
+  simp [bitmangling]
+  generalize List.range' 0 (Spec.w 6) = ls
+  induction ls generalizing res
+  case nil => simp
+  case cons hd tl ih => simp [ih]
 
-    simp [*, Spec.Keccak.ρ.inner_loop, Nat.mod_eq_of_lt]
-    simp_lists [List.drop_eq_getElem_cons]
-    -- simp [Fin.cast_of_mk]
-    congr 3
-    zmodify
-    ring
-  case isFalse =>
-    simp [‹z.val = Spec.w 6›']
-    simp_lists
-termination_by Spec.w 6 - z.val
-decreasing_by scalar_decr_tac
+theorem List.range'_advance_left: len > 0 → List.range' start len = start :: List.range' (start + 1) (len - 1) := by 
+  intros
+  have ⟨n, n_val⟩ := Nat.exists_add_one_eq.mpr ‹len > 0›
+  simp only [←n_val]
+  rfl
+
+theorem List.range'_advance_right: len > 0 → List.range' start len = List.range' start (len - 1) ++ [start + len - 1] := by 
+  intros
+  have ⟨n, n_val⟩ := Nat.exists_add_one_eq.mpr ‹len > 0›
+  simp only [←n_val, List.range'_concat]
+  simp
+
+theorem length_fold_set[Inhabited β](init: List β)(ls: List α)
+  (idx_f: α → Nat)
+  (value_f: α → β)
+: (List.foldl (fun b a => b.set (idx_f a) (value_f a)) (init := init) ls).length = init.length
+:= by induction ls generalizing init <;> simp [*]
+
+theorem IR.rho.getElem!_bitmangling_pos.aux(state res: List Bool)(x y offset: Nat)(i: Nat)(len: Nat)
+  (x_lt: x < 5)
+  (y_lt: y < 5)
+  (i_lt: i < len)
+  (encoded_lt_res: encodeIndex x y i < res.length)
+  (encoded_lt_state: encodeIndex x y i < state.length)
+: (List.foldl (fun b a => b.set (encodeIndex x y a) state[encodeIndex x y ((a + Spec.w 6 - offset % Spec.w 6) % Spec.w 6)]!) res
+      (List.range' 0 len))[encodeIndex x y i]! =
+  state[encodeIndex x y ((i + Spec.w 6 - offset % Spec.w 6) % Spec.w 6)]!
+:= by
+  cases len
+  case zero => simp at i_lt
+  case succ len' =>
+    simp [List.range'_concat]
+    if cond: len' = i then
+      simp [cond]
+      rw [List.getElem!_set]
+      simp [length_fold_set, *]
+    else
+      simp [cond, List.getElem!_set_ne]
+      rw [IR.rho.getElem!_bitmangling_pos.aux (len := len')]
+      all_goals (first | assumption | omega)
+
+
+theorem IR.rho.getElem!_bitmangling_pos(state res: List Bool)(x y offset: Nat)(i: Nat)
+  (x_lt: x < 5)
+  (y_lt: y < 5)
+  (i_lt: i < Spec.w 6)
+  (len_state: state.length = Spec.b 6)
+  (len_res: res.length = Spec.b 6)
+: (bitmangling state res x y offset)[IR.encodeIndex x y i]! = state[IR.encodeIndex x y ((i +  Spec.w 6 - offset % Spec.w 6) % Spec.w 6)]!
+:= by
+  have encoded_idx: IR.encodeIndex x y i < res.length := by
+    simp [encodeIndex, len_res]
+    scalar_tac
+  have encoded_idx: IR.encodeIndex x y i < state.length := by
+    simp [encodeIndex, len_state]
+    scalar_tac
+  simp [bitmangling]
+  rw [IR.rho.getElem!_bitmangling_pos.aux (len := Spec.w 6)]
+  all_goals assumption
+
+theorem IR.rho.getElem!_bitmangling_neg.aux(state res: List Bool)(x y offset: Nat)(i: Nat)(len: Nat)
+  (x_lt: x < 5)
+  (y_lt: y < 5)
+  (x'_lt: x' < 5)
+  (y'_lt: y' < 5)
+  (i_lt: i < Spec.w 6)
+  (len_lt: len ≤ Spec.w 6)
+  (encoded_lt_res: encodeIndex x y i < res.length)
+  (encoded_lt_state: encodeIndex x y i < state.length)
+  (ineq: ¬ (x' = x ∧ y' = y))
+: (List.foldl (fun b a => b.set (encodeIndex x y a) state[encodeIndex x y ((a + Spec.w 6 - offset % Spec.w 6) % Spec.w 6)]!) res
+      (List.range' 0 len))[encodeIndex x' y' i]! =
+  res[encodeIndex x' y' i]!
+:= by
+  cases len
+  case zero => simp [*]
+  case succ len' =>
+    simp [List.range'_concat]
+    have: encodeIndex x y len' ≠ encodeIndex x' y' i := by
+      apply IR.encode_eq_encode_iff_eq x x' y y' len' i x_lt y_lt (by omega) x'_lt y'_lt (by omega) |>.not.mpr
+      intro; simp at *; omega
+    rw [List.getElem!_set_neg]
+    case a => simp [this]
+    rw [aux]
+    all_goals (first | assumption | omega)
+
+theorem IR.rho.getElem!_bitmangling_neg(state res: List Bool)(x x' y y' offset: Nat)(i: Nat)
+  (x_lt: x < 5)
+  (y_lt: y < 5)
+  (x'_lt: x' < 5)
+  (y'_lt: y' < 5)
+  (i_lt: i < Spec.w 6)
+  (len_state: state.length = Spec.b 6)
+  (len_res: res.length = Spec.b 6)
+: ¬ (x' = x ∧ y' = y) → (bitmangling state res x y offset)[IR.encodeIndex x' y' i]! = res[encodeIndex x' y' i]!
+:= by
+  intro neq
+  have encoded_idx: IR.encodeIndex x y i < res.length := by
+    simp [encodeIndex, len_res]
+    scalar_tac
+  have encoded_idx: IR.encodeIndex x y i < state.length := by
+    simp [encodeIndex, len_state]
+    scalar_tac
+  simp [bitmangling]
+  rw [IR.rho.getElem!_bitmangling_neg.aux (len := Spec.w 6)]
+  all_goals (first | assumption | simp)
+
+def IR.rho.loop(state res: List Bool)(offset: Nat := 0)(x_init: Nat := 1)(y_init: Nat := 0): List Bool := Id.run do
+  let mut (x, y) := (x_init, y_init)
+  let mut res := res
+  for t in [offset:24] do
+    res := bitmangling state res x y (@Spec.Keccak.ρ.offset 6 t)
+    (x, y) := (y, (2*x + 3*y) % 5)
+  return res
+
+attribute [-simp] Aeneas.Std.UScalarTy.U64_numBits_eq
+
+theorem algos.rho.bitmangling.spec(input state: List Std.U64)(x' y': Nat)(offset: Std.U32)(x y z: Nat)
+  (x'_lt: x' < 5)
+  (y'_lt: y' < 5)
+  (x_lt: x < 5)
+  (y_lt: y < 5)
+  (z_lt: z < Spec.w 6)
+  (len_state: state.length = 25)
+  (len_res: input.length = 25)
+: (state.set (5 * y' + x') (Std.core.num.U64.rotate_left input[5 * y' + x']! offset)).toBits[IR.encodeIndex x y z]! 
+= (IR.rho.bitmangling input.toBits state.toBits x' y' offset.val)[IR.encodeIndex x y z]!
+:= by
+  have: 5 * y + x < 25 := Nat.lt_packing_right x_lt y_lt
+  if cond: x = x' ∧ y = y' then
+    rcases cond with ⟨rfl, rfl⟩
+    rw [IR.rho.getElem!_bitmangling_pos]
+    all_goals (first | simp [*, List.length_toBits, Spec.b, Spec.w]; done | try scalar_tac)
+    have: ((z + Spec.w 6 - ↑offset % Spec.w 6) % Spec.w 6) < Spec.w 6 := by simp [Nat.mod_lt, Spec.w]
+    simp [List.getElem!_toBits, IR.encodeIndex_xy, IR.encodeIndex_z, *, Std.core.num.U64.rotate_left]
+    /- rw [List.getElem!_set]; case h => simp [len_state, *] -/
+    /- rw [Aeneas.Std.U64.getElem!_toBits_rotate_left]; case i_idx => simp [Nat.mod_lt, Spec.w] -/
+    simp_lists 
+    simp only [Nat.mod_eq_of_lt, *]
+    simp [Spec.w]
+  else
+    rw [IR.rho.getElem!_bitmangling_neg]
+    all_goals (first | simp [*, List.length_toBits, Spec.b]; done | try scalar_tac)
+    have: 5*y' + x' ≠ 5 * y + x := by omega
+    simp [List.getElem!_toBits, IR.encodeIndex_xy, z_lt, this]
 
 @[progress]
-theorem algos.rho_loop.spec(input: algos.StateArray)
-(x y : Std.Usize) (res: algos.StateArray) (t: Std.Usize)
+theorem algos.rho_loop.spec(input res : StateArray) (x y : Std.Usize) (t: Std.U32)
 : t.val <= 24
 → x.val < 5
 → y.val < 5
 → ∃ output,
   rho_loop input x y res t = .ok output ∧
-  output.toSpec = Spec.Keccak.ρ.loop input.toSpec res.toSpec t.val.cast x.val.cast y.val.cast
+  output.toBits = IR.rho.loop input.toBits res.toBits t.val x.val y.val
 := by
-  intro t_loop_bnd x_idx y_idx
+  intro t_lt x_lt y_lt
   rw [rho_loop]
-  split
-  case isTrue t_lt =>
-    let* ⟨ res1, res1_post ⟩ ← rho.inner_loop.spec
-    let* ⟨ i, i_post ⟩ ← Std.Usize.mul_spec
-    let* ⟨ i1, i1_post ⟩ ← Std.Usize.mul_spec
-    let* ⟨ i2, i2_post ⟩ ← Std.Usize.add_spec
-    let* ⟨ lhs, lhs_post ⟩ ← Std.Usize.rem_spec
-    let* ⟨ t1, t1_post ⟩ ← Std.Usize.add_spec
-    let* ⟨ rest, rest_post ⟩ ← spec input
-
-    simp [*, Spec.Keccak.ρ.loop]
-    simp_lists [List.drop_eq_getElem_cons]
-    congr 4
-    zmodify [Fin.val_ofNat]
+  progress*
+  · simp only [*, Std.Array.toBits]
+    simp only [IR.rho.loop, Id.run, Fin.isValue, Id.pure_eq, Id.bind_eq,
+      Std.Range.forIn_eq_forIn_range', Std.Range.size, List.forIn_yield_eq_foldl]
+    simp only [Nat.sub_zero, Nat.add_sub_cancel, Nat.div_one, Nat.reduceSubDiff]
+    simp only [List.range'_advance_left (show 24 - t.val > 0 from by scalar_tac)]
+    simp only [Fin.isValue, List.foldl_cons, Fin.val_natCast]
+    congr 2
+    · simp [*]
+      ext i
+      · simp [List.length_toBits, IR.rho.length_bitmangling]
+      assume i < Spec.b 6; 
+      case otherwise => 
+        rw [getElem!_neg]; case h => simp [List.length_toBits, Spec.w]; scalar_tac
+        rw [getElem!_neg]; case h => simp [IR.rho.length_bitmangling]; scalar_tac
+      have ⟨x', y', z', encode_xyz_def, x'_lt, y'_lt, z'_lt⟩:= IR.decode_surjective i (by assumption)
+      rw [←encode_xyz_def, algos.rho.bitmangling.spec]
+      all_goals (first | assumption | simp [*])
+    · congr 1; omega
   case isFalse =>
-    simp [‹t.val = 24›', Spec.Keccak.ρ.loop]
+    simp [IR.rho.loop, ‹t.val = 24›']
 termination_by 24 - t.val
 decreasing_by scalar_decr_tac
+
+def Spec.Keccak.ρ.loop.inner(A A': StateArray l)(x y : Fin 5)(t: Fin 24)(z: Nat := 0): StateArray l := Id.run do
+  let mut A' := A'
+  for z in List.finRange (w l) |>.drop z do
+    A' := A'.set x y z <| A.get x y (z - ρ.offset t)
+  return A'
+
+/- example(ls: List α)(n: Nat): n < ls.length → ls.drop n = ls[n] :: ls.drop (n + 1) := by exact -/
+/-   fun a => List.drop_eq_getElem_cons sorry -/
+
+/- theorem apply_foldl(ls: List α)(init: β)(upd: β → α → β)(f: β → β')⦃g: β' → β⦄ -/
+/-   (leftInv: Function.LeftInverse g f) -/
+/- : f (ls.foldl upd init) = ls.foldl (fun acc i => f $ upd (g acc) i) (f init) -/
+/- := by -/
+/-   induction ls using List.reverseRecOn -/
+/-   case nil => simp only [List.foldl_nil] -/
+/-   case append_singleton preffix last ih => -/
+/-     simp only [Function.LeftInverse] at leftInv -/
+/-     simp [←ih, leftInv] -/
+
+/- @[simp] -/
+/- theorem List.drop_pmap.{u_1, u_2} {α : Type u_1} {β : Type u_2} {P : α → Prop} (f : (a : α) → P a → β) (l : List α) -/
+/-   (H : ∀ a ∈ l, P a)(n: Nat) -/
+/- : (List.pmap f l H).drop n = List.pmap f (l.drop n) (fun x x_in_drop => H x (List.mem_of_mem_drop x_in_drop)) -/
+/- := by ext i : 1; simp -/
+
+/- #check (show ∀ x ∈ List.range' 0 (Spec.w 6), x < Spec.w 6 from by intro x x_in; simpa using x_in) -/
+/- #check -- ∀ x ∈ List.range' 0 (Spec.w 6), x < Spec.w 6 -/
+/-   List.finRange (Spec.w 6) -/ 
+/- #check List.range' 0 (Spec.w 6) |>.pmap Fin.mk (by intro x x_in; simpa using x_in) -/
+
+/- theorem foldl_spec{ι₀ ι₁ α₀ α₁} -/
+/-   {ls0: List ι₀}{upd0: α₀ → ι₀ → α₀}{init0: α₀} -/
+/-   {ls1: List ι₁}{upd1: α₁ → ι₁ → α₁}{init1: α₁} -/
+/-   (inv : α₀ → α₁ → Prop) -/
+/-   (idx_rel : ι₀ → ι₁ → Prop) -/
+/-   (pre: inv init0 init1) -/
+/-   (eq_length: ls0.length = ls1.length) -/
+/-   (step: ∀ {i: Nat} (_: i < ls0.length), idx_rel ls0[i] ls1[i] →  ∀ a0 a1, inv a0 a1 → inv (upd0 a0 ls0[i]) (upd1 a1 ls1[i])) -/
+/- : inv (ls0.foldl upd0 init0) (ls1.foldl upd1 init1) -/
+/- := by -/
+/-   sorry -/
+
+/- theorem foldl_range{ls: List ι}{upd: α → ι → α}{init: α} -/
+/- : ls.foldl upd init = (List.range' 0 ls.length).attach.foldl (fun a (i: {x // x ∈ List.range' 0 ls.length}) => -/
+/-     have: i.val < ls.length := by simpa using i.property -/
+/-     upd a ls[i.val]) init -/
+/- := by -/ 
+/-   sorry -/
+
+/- theorem foldl_finRange{ls: List ι}{upd: α → ι → α}{init: α} -/
+/- : ls.foldl upd init = (List.finRange ls.length).foldl (fun a i => upd a ls[i]) init -/
+/- := by -/ 
+/-   sorry -/
+
+/- theorem foldl_finRange_step{ls: List ι}{upd: α → Fin (ls.length) → α}{init: α}(i: Nat) -/
+/- : (List.finRange ls.length |>.drop i).foldl upd = if i < ls.length then (List.finRange ls.length |>.drop (i + 1)).foldl upd -/
+/- := by -/ 
+/-   sorry -/
+
+/- theorem foldl_step{ls: List ι}{upd: α → ι → α}{init: α} -/
+/- : ls.foldl upd init = (List.range' 0 ls.length).attach.foldl (fun a (i: {x // x ∈ List.range' 0 ls.length}) => -/
+/-     have: i.val < ls.length := by simpa using i.property -/
+/-     upd a ls[i.val]) init -/
+/- := by -/ 
+/-   sorry -/
+
+theorem IR.rho.bitmangling.step(state res: List Bool)(x y offset: Nat)(z: Nat)
+: bitmangling state res x y offset z = 
+  if z < Spec.w 6 then 
+    let res := res.set (IR.encodeIndex x y z) <| state[IR.encodeIndex x y ((z + Spec.w 6 - offset % Spec.w 6) % Spec.w 6)]!
+    bitmangling state res x y offset (z + 1)
+  else res
+:= by
+  simp [bitmangling]
+  if cond: z < Spec.w 6 then
+    simp [cond, List.range'_advance_left, Nat.sub_add_eq]
+  else
+    simp [cond, not_lt.mp cond, Nat.sub_eq_zero_of_le]
+
+theorem Spec.Keccak.ρ.loop.inner.step(A A': Spec.Keccak.StateArray 6)(x y : Fin 5)(t: Fin 24)(z: Nat)
+: Spec.Keccak.ρ.loop.inner A A' x y t z = 
+    if z < Spec.w 6 then 
+      let A' := A'.set x y z <| A.get x y (z.cast - ρ.offset t)
+      Spec.Keccak.ρ.loop.inner A A' x y t (z + 1)
+    else
+      A'
+:= by
+  simp [inner]
+  if cond: z < Spec.w 6 then
+    simp [cond, ←List.cons_getElem_drop_succ, Fin.natCast_def, Nat.mod_eq_of_lt]
+  else
+    simp [cond, not_lt.mp]
+  
+theorem IR.rho.bitmangling.refinement'(A A': Spec.Keccak.StateArray 6)(x y : Fin 5)(t: Fin 24)(z: Nat)
+: (Spec.Keccak.ρ.loop.inner A A' x y t z).toBits = IR.rho.bitmangling A.toBits A'.toBits x.val y.val (@Spec.Keccak.ρ.offset 6 t) z
+:= by
+  rw [bitmangling.step, Spec.Keccak.ρ.loop.inner.step]
+  split
+  · simp [*]
+    rw [IR.rho.bitmangling.refinement']
+    congr
+    -- TODO: This should be a theorem, toBits_set or something like that.
+    simp +arith +decide [Spec.Keccak.StateArray.set, Spec.Keccak.StateArray.get, Spec.Keccak.StateArray.toBits, Spec.Keccak.StateArray.toBitsSubtype,
+      Spec.Keccak.StateArray.encodeIndex, encodeIndex, Nat.mod_eq_of_lt, *, Spec.Keccak.ρ.offset, Fin.val_sub, ←getElem!_pos]
+    rw [Nat.add_sub_assoc]
+    case h => simp +decide [le_of_lt, Nat.mod_lt]
+  · rfl
+
+/- theorem IR.rho.bitmangling.refinement(A A': Spec.Keccak.StateArray 6)(x y : Fin 5)(t: Fin 24)(z: Nat) -/
+/- : (Spec.Keccak.ρ.loop.inner A A' x y t z).toBits = IR.rho.bitmangling A.toBits A'.toBits x.val y.val (@Spec.Keccak.ρ.offset 6 t) z -/
+/- := by -/
+/-   simp only [Fin.isValue, Spec.Keccak.ρ.loop.inner, Id.run, Id.pure_eq, Id.bind_eq, -/
+/-     List.forIn_yield_eq_foldl, bitmangling, Array.getElem!_toList, Vector.getElem!_toArray, -/
+/-     Std.Range.forIn_eq_forIn_range', Std.Range.size, add_tsub_cancel_right, Nat.div_one] -/
+/-   /1- have: List.finRange (Spec.w 6) = (List.range' 0 (Spec.w 6)).pmap Fin.mk (by intro x x_in; simpa using x_in) := by simp +decide -1/ -/
+/-   /1- rw [this] -1/ -/
+
+/-   generalize upd_def: (fun acc i => -/
+/-     (Spec.Keccak.StateArray.set x y i (Spec.Keccak.StateArray.get x y (i - Spec.Keccak.ρ.offset t.val) A) acc)) = upd -/
+/-   generalize upd'_def: (fun (b: List Bool) (a: Nat) => -/
+/-     b.set (encodeIndex x.val (y.val) a) A.toVector[encodeIndex (x.val) (y.val) ((a + Spec.w 6 - (Spec.Keccak.ρ.offset ↑t).val % Spec.w 6) % Spec.w 6)]!) = upd' -/
+
+/-   rw [apply_foldl (leftInv := Spec.Keccak.StateArray.LeftInverse_toBits)] -/
+/-   simp [List.finRange_eq_pmap_range, List.pmap_eq_map, List.foldl_pmap] -/
+/-   rw [List.foldl_subtype, List.unattach_attach, List.range_eq_range', List.drop_range', Nat.zero_add] -/
+/-   intro st z' z'_in -/
+/-   simp only [Fin.isValue, ←upd_def, ←upd'_def] -/
+/-   open Spec.Keccak in simp only [StateArray.set, StateArray.get, StateArray.toBits, StateArray.encodeIndex, encodeIndex] -/
+/-   unfold List.toStateArray -/
+/-   simp [List.range_eq_range', List.drop_range'] at z'_in -/
+/-   have: z' < Spec.w 6 := by omega -/
+/-   simp [Fin.val_sub, (Spec.Keccak.ρ.offset t.val).isLt, Nat.mod_eq_of_lt] -/
+/-   -- TODO: I need to carry the property that the list has length 1600 up to here, somehow -/
+/-   split -/
+/-   · simp +arith [Nat.add_sub_assoc, (Spec.Keccak.ρ.offset t.val).isLt, le_of_lt, ←getElem!_pos] -/
+/-   · sorry -/
+
+def Spec.Keccak.ρ.loop(A: StateArray l)(A': StateArray l := A)(x : Fin 5 := 1)(y : Fin 5 := 0)(offset: Nat := 0): StateArray l := Id.run do
+  let mut (x, y): Fin 5 × Fin 5 := (x,y)
+  let mut A' := A'
+  for t in List.finRange 24 |>.drop offset do
+    A' := Spec.Keccak.ρ.loop.inner A A' x y t 
+    (x, y) := (y, 2*x + 3*y)
+  return A'
+
+theorem Spec.Keccak.ρ.loop.step(A A': StateArray l)(x y : Fin 5)(t: Nat)
+: loop A A' x y t = 
+    if t < 24 then 
+      let A' := Spec.Keccak.ρ.loop.inner A A' x y t
+      let (x,y) := (y, 2*x + 3*y)
+      loop A A' x y (t + 1)
+    else
+      A'
+:= by
+  simp [loop]
+  if cond: t < 24 then
+    simp [cond, ←List.cons_getElem_drop_succ, Fin.natCast_def, Nat.mod_eq_of_lt]
+  else
+    simp [cond, not_lt.mp]
+
+theorem IR.rho.loop.step(state res: List Bool)(t x y: Nat)
+: loop state res t x y = 
+    if t < 24 then
+      let res := bitmangling state res x y (@Spec.Keccak.ρ.offset 6 t)
+      let (x, y) := (y, (2*x + 3*y) % 5)
+      loop state res (t + 1) x y
+    else
+      res
+:= by
+  simp [loop]
+  if cond: t < 24 then
+    simp +arith [cond, List.range'_advance_left, Nat.sub_right_comm 24 t]
+  else
+    simp [cond, List.range'_eq_nil_iff.mpr, Nat.sub_eq_zero_of_le, not_lt.mp]
+
+/- private theorem List.foldl_congr{ls ls': List α} -/
+/- : ls = ls' -/
+/- → upd = upd' -/
+/- → init = init' -/
+/- → ls.foldl upd init = ls'.foldl upd' init' -/
+/- := by rintro rfl rfl rfl; rfl -/
+
+/- theorem toBits_foldl(ls: List α)(init: Spec.Keccak.StateArray 6)(upd: _) -/
+/- : let upd' (acc: {ls: List Bool // ls.length = 1600})(i: α):= { val := (upd (acc.val.toStateArray (by simp)) i).toBits, property := by simp +decide} -/
+/-   let init': {ls: List Bool // ls.length = 1600} := { -/
+/-     val := init.toBits -/
+/-     property := by simp +decide -/
+/-   } -/
+/-   (ls.foldl upd init).toBits = -/ 
+/-   ls.foldl  (fun acc i => upd' acc i) init' -/
+/- := by -/
+/-   sorry -/
+
+theorem Spec.Keccak.ρ.unfold(A: StateArray l)
+: ρ A = ρ.loop A
+:= by congr
+
+theorem IR.rho.loop.refinement'(state res: Spec.Keccak.StateArray 6)(x y: Fin 5)(t: Nat)
+: (Spec.Keccak.ρ.loop state res x y t).toBits = IR.rho.loop state.toBits res.toBits t x.val y.val
+:= by
+  /- sorry -/
+  rw [Spec.Keccak.ρ.loop.step, IR.rho.loop.step]
+  if cond: t < 24 then
+    simp only [cond, ↓reduceIte, Fin.isValue]
+    rw [IR.rho.loop.refinement']
+    simp only [cond, bitmangling.refinement', Nat.mod_eq_of_lt, Fin.val_add, Fin.val_mul, Fin.natCast_def]
+    congr 1
+    zmodify
+  else
+    simp [cond]
+termination_by 24 - t
 
 @[progress]
 theorem algos.rho.spec(input: algos.StateArray)
 : ∃ output,
-  algos.rho input = .ok output ∧ output.toSpec = Spec.Keccak.ρ input.toSpec
+  algos.rho input = .ok output ∧ output.toBits = (Spec.Keccak.ρ input.toSpec).toBits
 := by
   /- rw [Spec.Keccak.ρ.loop] -/
-  simp [rho, ClonealgosStateArray.clone]
-  progress as ⟨res, res_post⟩
-  simp [res_post, Spec.Keccak.ρ.loop.spec]
+  simp [rho, Spec.Keccak.ρ.unfold]
+  progress with rho_loop.spec as ⟨ res, res_post ⟩
+  simp +decide [*, IR.rho.loop.refinement', List.toBits_toStateArray]
+  
